paper/WIP/proof/kernel/kernel.ml
@@ -1,0 +1,603 @@
+
+(** val negb : bool -> bool **)
+
+let negb = function
+| true -> false
+| false -> true
+
+(** val fst : ('a1 * 'a2) -> 'a1 **)
+
+let fst = function
+| (x, _) -> x
+
+(** val snd : ('a1 * 'a2) -> 'a2 **)
+
+let snd = function
+| (_, y) -> y
+
+(** val length : 'a1 list -> int **)
+
+let rec length = function
+| [] -> 0
+| _ :: l' -> Stdlib.Int.succ (length l')
+
+(** val app : 'a1 list -> 'a1 list -> 'a1 list **)
+
+let rec app l m =
+  match l with
+  | [] -> m
+  | a :: l1 -> a :: (app l1 m)
+
+(** val bool_dec : bool -> bool -> bool **)
+
+let bool_dec b1 b2 =
+  if b1 then if b2 then true else false else if b2 then false else true
+
+module Nat =
+ struct
+ end
+
+(** val in_dec : ('a1 -> 'a1 -> bool) -> 'a1 -> 'a1 list -> bool **)
+
+let rec in_dec h a = function
+| [] -> false
+| y :: l0 -> let s = h y a in if s then true else in_dec h a l0
+
+(** val nth : int -> 'a1 list -> 'a1 -> 'a1 **)
+
+let rec nth n l default =
+  (fun fO fS n -> if n=0 then fO () else fS (n-1))
+    (fun _ -> match l with
+              | [] -> default
+              | x :: _ -> x)
+    (fun m -> match l with
+              | [] -> default
+              | _ :: t -> nth m t default)
+    n
+
+(** val concat : 'a1 list list -> 'a1 list **)
+
+let rec concat = function
+| [] -> []
+| x :: l0 -> app x (concat l0)
+
+(** val list_eq_dec : ('a1 -> 'a1 -> bool) -> 'a1 list -> 'a1 list -> bool **)
+
+let rec list_eq_dec eq_dec l l' =
+  match l with
+  | [] -> (match l' with
+           | [] -> true
+           | _ :: _ -> false)
+  | y :: l0 ->
+    (match l' with
+     | [] -> false
+     | a :: l1 -> if eq_dec y a then list_eq_dec eq_dec l0 l1 else false)
+
+(** val map : ('a1 -> 'a2) -> 'a1 list -> 'a2 list **)
+
+let rec map f0 = function
+| [] -> []
+| a :: t -> (f0 a) :: (map f0 t)
+
+(** val existsb : ('a1 -> bool) -> 'a1 list -> bool **)
+
+let rec existsb f0 = function
+| [] -> false
+| a :: l0 -> (||) (f0 a) (existsb f0 l0)
+
+(** val filter : ('a1 -> bool) -> 'a1 list -> 'a1 list **)
+
+let rec filter f0 = function
+| [] -> []
+| x :: l0 -> if f0 x then x :: (filter f0 l0) else filter f0 l0
+
+(** val find : ('a1 -> bool) -> 'a1 list -> 'a1 option **)
+
+let rec find f0 = function
+| [] -> None
+| x :: tl -> if f0 x then Some x else find f0 tl
+
+(** val list_prod : 'a1 list -> 'a2 list -> ('a1 * 'a2) list **)
+
+let rec list_prod l l' =
+  match l with
+  | [] -> []
+  | x :: t -> app (map (fun y -> (x, y)) l') (list_prod t l')
+
+(** val seq : int -> int -> int list **)
+
+let rec seq start len =
+  (fun fO fS n -> if n=0 then fO () else fS (n-1))
+    (fun _ -> [])
+    (fun len0 -> start :: (seq (Stdlib.Int.succ start) len0))
+    len
+
+(** val repeat : 'a1 -> int -> 'a1 list **)
+
+let rec repeat x n =
+  (fun fO fS n -> if n=0 then fO () else fS (n-1))
+    (fun _ -> [])
+    (fun k -> x :: (repeat x k))
+    n
+
+type role = int
+
+type capN = int
+
+type lab = int
+
+(** val add_new : ('a1 -> 'a1 -> bool) -> 'a1 list -> 'a1 list -> 'a1 list **)
+
+let rec add_new a_dec s = function
+| [] -> s
+| x :: t -> add_new a_dec (if in_dec a_dec x s then s else x :: s) t
+
+(** val expand' :
+    ('a1 -> 'a1 -> bool) -> ('a1 -> 'a1 list) -> 'a1 list -> 'a1 list **)
+
+let expand' a_dec succ s =
+  add_new a_dec s (concat (map succ s))
+
+(** val iter' :
+    ('a1 -> 'a1 -> bool) -> ('a1 -> 'a1 list) -> int -> 'a1 list -> 'a1 list **)
+
+let rec iter' a_dec succ n s =
+  (fun fO fS n -> if n=0 then fO () else fS (n-1))
+    (fun _ -> s)
+    (fun k ->
+    let s' = expand' a_dec succ s in
+    if (=) (length s') (length s) then s else iter' a_dec succ k s')
+    n
+
+(** val decide' :
+    ('a1 -> 'a1 -> bool) -> ('a1 -> 'a1 list) -> 'a1 list -> ('a1 -> bool) ->
+    'a1 -> bool **)
+
+let decide' a_dec succ all hb x =
+  existsb hb (iter' a_dec succ (length all) (x :: []))
+
+type ('node, 'w) pS' = ('node * 'w) * int
+
+(** val ps_dec :
+    ('a1 -> 'a1 -> bool) -> ('a2 -> 'a2 -> bool) -> ('a1, 'a2) pS' -> ('a1,
+    'a2) pS' -> bool **)
+
+let ps_dec node_dec w_dec x y =
+  let (a, b) = x in
+  let (p, n) = y in
+  if let (a0, b0) = a in
+     let (n0, w) = p in if node_dec a0 n0 then w_dec b0 w else false
+  then (=) b n
+  else false
+
+(** val psucc :
+    ('a1 -> 'a2 -> ('a1 * 'a2) list) -> ('a1 -> 'a2 -> ('a1 * 'a2) list) ->
+    ('a1, 'a2) pS' -> ('a1, 'a2) pS' list **)
+
+let psucc succ2 succ3 = function
+| (p, b) ->
+  let (n, w) = p in
+  app (map (fun p0 -> (((fst p0), (snd p0)), b)) (succ2 n w))
+    ((fun fO fS n -> if n=0 then fO () else fS (n-1))
+       (fun _ -> [])
+       (fun b' -> map (fun p0 -> (((fst p0), (snd p0)), b')) (succ3 n w))
+       b)
+
+(** val upto : int -> int list **)
+
+let rec upto k =
+  (fun fO fS n -> if n=0 then fO () else fS (n-1))
+    (fun _ -> 0 :: [])
+    (fun k' -> (Stdlib.Int.succ k') :: (upto k'))
+    k
+
+(** val all_ps : 'a1 list -> 'a2 list -> int -> ('a1, 'a2) pS' list **)
+
+let all_ps nodes worlds k =
+  concat
+    (map (fun n ->
+      concat (map (fun w -> map (fun b -> ((n, w), b)) (upto k)) worlds))
+      nodes)
+
+(** val phazb : ('a2 -> bool) -> ('a1, 'a2) pS' -> bool **)
+
+let phazb hazb0 = function
+| (p, _) -> let (_, w) = p in hazb0 w
+
+(** val decide_reachb_fast :
+    ('a1 -> 'a1 -> bool) -> ('a2 -> 'a2 -> bool) -> 'a1 list -> 'a2 list ->
+    ('a1 -> 'a2 -> ('a1 * 'a2) list) -> ('a1 -> 'a2 -> ('a1 * 'a2) list) ->
+    ('a2 -> bool) -> int -> 'a1 -> 'a2 -> bool **)
+
+let decide_reachb_fast node_dec w_dec nodes worlds succ2 succ3 hazb0 k n w =
+  decide' (ps_dec node_dec w_dec) (psucc succ2 succ3) (all_ps nodes worlds k)
+    (phazb hazb0) ((n, w), k)
+
+type 'gd gr =
+| REnd
+| RComm of role * role * ((lab * 'gd) * 'gd gr) list
+| RAct of capN * role * 'gd gr
+| RGoal of 'gd * 'gd gr
+| RMu of 'gd gr
+| RVar of int
+
+(** val gr_rect_list :
+    'a2 -> (role -> role -> ((lab * 'a1) * 'a1 gr) list -> 'a3 -> 'a2) ->
+    (capN -> role -> 'a1 gr -> 'a2 -> 'a2) -> ('a1 -> 'a1 gr -> 'a2 -> 'a2)
+    -> ('a1 gr -> 'a2 -> 'a2) -> (int -> 'a2) -> 'a3 -> (((lab * 'a1) * 'a1
+    gr) -> ((lab * 'a1) * 'a1 gr) list -> 'a2 -> 'a3 -> 'a3) -> 'a1 gr -> 'a2 **)
+
+let rec gr_rect_list hEnd hComm hAct hGoal hMu hVar hnil hcons = function
+| REnd -> hEnd
+| RComm (p, q, brs) ->
+  hComm p q brs
+    (let rec f0 = function
+     | [] -> hnil
+     | b :: bs' ->
+       hcons b bs'
+         (gr_rect_list hEnd hComm hAct hGoal hMu hVar hnil hcons (snd b))
+         (f0 bs')
+     in f0 brs)
+| RAct (a, p, g0) ->
+  hAct a p g0 (gr_rect_list hEnd hComm hAct hGoal hMu hVar hnil hcons g0)
+| RGoal (g0, g1) ->
+  hGoal g0 g1 (gr_rect_list hEnd hComm hAct hGoal hMu hVar hnil hcons g1)
+| RMu g0 -> hMu g0 (gr_rect_list hEnd hComm hAct hGoal hMu hVar hnil hcons g0)
+| RVar n -> hVar n
+
+type 'gd env = 'gd gr option list
+
+(** val subst : 'a1 env -> 'a1 gr -> 'a1 gr **)
+
+let rec subst rho = function
+| REnd -> REnd
+| RComm (p, q, brs) ->
+  RComm (p, q,
+    (map (fun b -> (((fst (fst b)), (snd (fst b))), (subst rho (snd b)))) brs))
+| RAct (a, p, g0) -> RAct (a, p, (subst rho g0))
+| RGoal (g0, g1) -> RGoal (g0, (subst rho g1))
+| RMu g0 -> RMu (subst (None :: rho) g0)
+| RVar n -> (match nth n rho None with
+             | Some m -> m
+             | None -> RVar n)
+
+(** val unfold_mu : 'a1 gr -> 'a1 gr **)
+
+let unfold_mu g0 =
+  subst ((Some (RMu g0)) :: []) g0
+
+(** val close : 'a1 gr list -> 'a1 gr -> 'a1 gr **)
+
+let close ctx g =
+  subst (map (fun x -> Some x) ctx) g
+
+(** val cands : 'a1 gr list -> 'a1 gr -> 'a1 gr list **)
+
+let rec cands ctx g =
+  (close ctx g) :: (match g with
+                    | RComm (_, _, brs) ->
+                      concat (map (fun b -> cands ctx (snd b)) brs)
+                    | RAct (_, _, g0) -> cands ctx g0
+                    | RGoal (_, g0) -> cands ctx g0
+                    | RMu g0 -> cands ((close ctx (RMu g0)) :: ctx) g0
+                    | _ -> [])
+
+(** val gr_eq_dec : ('a1 -> 'a1 -> bool) -> 'a1 gr -> 'a1 gr -> bool **)
+
+let gr_eq_dec gd_dec0 =
+  gr_rect_list (fun g2 -> match g2 with
+                          | REnd -> true
+                          | _ -> false) (fun p q _ hl g2 ->
+    match g2 with
+    | RComm (r, r0, l) ->
+      let s = (=) p r in
+      if s then let s0 = (=) q r0 in if s0 then hl l else false else false
+    | _ -> false) (fun a p _ iH g2 ->
+    match g2 with
+    | RAct (c, r, g) ->
+      let s = (=) a c in
+      if s then let s0 = (=) p r in if s0 then iH g else false else false
+    | _ -> false) (fun g _ iH g2 ->
+    match g2 with
+    | RGoal (g0, g1) -> let s = gd_dec0 g g0 in if s then iH g1 else false
+    | _ -> false) (fun _ iH g2 -> match g2 with
+                                  | RMu g -> iH g
+                                  | _ -> false) (fun n g2 ->
+    match g2 with
+    | RVar n0 -> (=) n n0
+    | _ -> false) (fun brs' -> match brs' with
+                               | [] -> true
+                               | _ :: _ -> false) (fun b _ hb hbs brs' ->
+    let (p, _) = b in
+    let (l, g) = p in
+    (match brs' with
+     | [] -> false
+     | p0 :: l0 ->
+       let (p1, g0) = p0 in
+       let (l1, g1) = p1 in
+       let s = (=) l l1 in
+       if s
+       then let s0 = gd_dec0 g g1 in
+            if s0
+            then let s1 = hb g0 in if s1 then hbs l0 else false
+            else false
+       else false))
+
+(** val succ0 :
+    ('a2 -> 'a1 -> bool) -> (capN -> 'a1 -> 'a1 list) -> 'a2 gr -> 'a1 ->
+    ('a2 gr * 'a1) list **)
+
+let succ0 satb0 succE0 g w =
+  match g with
+  | RComm (_, _, brs) ->
+    map (fun b -> ((snd b), w)) (filter (fun b -> satb0 (snd (fst b)) w) brs)
+  | RAct (a, _, g0) -> map (fun w' -> (g0, w')) (succE0 a w)
+  | RGoal (_, g0) -> (g0, w) :: []
+  | RMu g0 -> ((unfold_mu g0), w) :: []
+  | _ -> []
+
+(** val succ1 :
+    ('a2 -> 'a1 -> bool) -> 'a2 gr -> 'a1 -> ('a2 gr * 'a1) list **)
+
+let succ1 satb0 g w =
+  match g with
+  | RComm (_, _, brs) ->
+    map (fun b -> ((snd b), w))
+      (filter (fun b -> negb (satb0 (snd (fst b)) w)) brs)
+  | _ -> []
+
+(** val decide_mu :
+    ('a1 -> 'a1 -> bool) -> ('a2 -> 'a2 -> bool) -> 'a1 list -> ('a2 -> 'a1
+    -> bool) -> (capN -> 'a1 -> 'a1 list) -> ('a1 -> bool) -> int -> 'a2 gr
+    -> 'a1 -> bool **)
+
+let decide_mu wd_dec0 gd_dec0 worlds satb0 succE0 hazb0 k g0 w =
+  decide_reachb_fast (gr_eq_dec gd_dec0) wd_dec0 (cands [] g0) worlds
+    (succ0 satb0 succE0) (succ1 satb0) hazb0 k g0 w
+
+type wd = bool list
+
+(** val wd_dec : wd -> wd -> bool **)
+
+let wd_dec =
+  list_eq_dec bool_dec
+
+(** val wd_eqb : wd -> wd -> bool **)
+
+let wd_eqb x y =
+  if wd_dec x y then true else false
+
+(** val wget : wd -> int -> bool **)
+
+let wget w i =
+  nth i w false
+
+(** val wset : wd -> int -> bool -> wd **)
+
+let rec wset w i v =
+  match w with
+  | [] -> []
+  | b :: t ->
+    ((fun fO fS n -> if n=0 then fO () else fS (n-1))
+       (fun _ -> v :: t)
+       (fun i' -> b :: (wset t i' v))
+       i)
+
+(** val set_all : bool -> int list -> wd -> wd **)
+
+let rec set_all v is w =
+  match is with
+  | [] -> w
+  | i :: t -> set_all v t (wset w i v)
+
+type f =
+| FTrue
+| FAtom of int
+| FAnd of f * f
+| FOr of f * f
+| FNot of f
+
+(** val satf : f -> wd -> bool **)
+
+let rec satf f0 w =
+  match f0 with
+  | FTrue -> true
+  | FAtom i -> wget w i
+  | FAnd (a, b) -> (&&) (satf a w) (satf b w)
+  | FOr (a, b) -> (||) (satf a w) (satf b w)
+  | FNot a -> negb (satf a w)
+
+type act = { a_pre : f; a_add : int list; a_del : int list; a_haz : wd list }
+
+(** val never : act **)
+
+let never =
+  { a_pre = (FNot FTrue); a_add = []; a_del = []; a_haz = [] }
+
+(** val apply_act : int -> act -> wd -> wd **)
+
+let apply_act hz a w =
+  let w2 = set_all false a.a_del (set_all true a.a_add w) in
+  if existsb (wd_eqb w2) a.a_haz then wset w2 hz true else w2
+
+(** val succE : int -> act list -> capN -> wd -> wd list **)
+
+let succE hz tbl a w =
+  let ac = nth a tbl never in
+  if satf ac.a_pre w then (apply_act hz ac w) :: [] else []
+
+(** val hazb : int -> wd -> bool **)
+
+let hazb hz w =
+  wget w hz
+
+type gd = wd list
+
+(** val gd_dec : gd -> gd -> bool **)
+
+let gd_dec =
+  list_eq_dec wd_dec
+
+(** val satb : gd -> wd -> bool **)
+
+let satb g w =
+  existsb (wd_eqb w) g
+
+(** val all_bits : int -> wd list **)
+
+let rec all_bits n =
+  (fun fO fS n -> if n=0 then fO () else fS (n-1))
+    (fun _ -> [] :: [])
+    (fun k ->
+    app (map (fun x -> true :: x) (all_bits k))
+      (map (fun x -> false :: x) (all_bits k)))
+    n
+
+(** val kernel_hazard :
+    int -> int -> act list -> int -> gd gr -> wd -> bool **)
+
+let kernel_hazard n hz tbl k g0 w0 =
+  decide_mu wd_dec gd_dec (all_bits n) satb (succE hz tbl) (hazb hz) k g0 w0
+
+(** val kernel_first :
+    int -> int -> act list -> int -> gd gr -> wd -> int option **)
+
+let kernel_first n hz tbl kmax g0 w0 =
+  find (fun k -> kernel_hazard n hz tbl k g0 w0)
+    (seq 0 (Stdlib.Int.succ kmax))
+
+type gW = gd gr * wd
+
+(** val gW_dec : gW -> gW -> bool **)
+
+let gW_dec x y =
+  let (g, w) = x in
+  let (g0, w0) = y in
+  let s = gr_eq_dec gd_dec g g0 in if s then wd_dec w w0 else false
+
+(** val gsucc : int -> act list -> gW -> gW list **)
+
+let gsucc hz tbl s =
+  app (succ0 satb (succE hz tbl) (fst s) (snd s)) (succ1 satb (fst s) (snd s))
+
+(** val is_end : gd gr -> bool **)
+
+let is_end = function
+| REnd -> true
+| _ -> false
+
+(** val goal_hit : f -> gW -> bool **)
+
+let goal_hit goal s =
+  (&&) (is_end (fst s)) (satf goal (snd s))
+
+(** val goal_reachable :
+    int -> int -> act list -> f -> gd gr -> wd -> bool **)
+
+let goal_reachable n hz tbl goal g w =
+  decide' gW_dec (gsucc hz tbl) (list_prod (cands [] g) (all_bits n))
+    (goal_hit goal) (g, w)
+
+type raw =
+| WEnd
+| WAct of int * bool * role * raw
+| WChoice of role * role * ((lab * f option) * raw) list
+| WMu of raw
+| WVar of int
+
+type bCap = { b_pre : f; b_add : int list; b_del : int list }
+
+(** val base_act : bCap -> act **)
+
+let base_act b =
+  { a_pre = b.b_pre; a_add = b.b_add; a_del = b.b_del; a_haz = [] }
+
+(** val never_b : bCap **)
+
+let never_b =
+  { b_pre = (FNot FTrue); b_add = []; b_del = [] }
+
+(** val skel : gd -> raw -> gd gr **)
+
+let rec skel all = function
+| WEnd -> REnd
+| WAct (c, _, p, g) -> RAct (c, p, (skel all g))
+| WChoice (p, q, brs) ->
+  RComm (p, q,
+    (map (fun b -> (((fst (fst b)), all), (skel all (snd b)))) brs))
+| WMu g -> RMu (skel all g)
+| WVar i -> RVar i
+
+type params = { p_n : int; p_hz : int; p_base : bCap list; p_goal : f;
+                p_worlds : wd list }
+
+(** val gr0 : params -> gd gr -> wd -> bool **)
+
+let gr0 p g w =
+  goal_reachable p.p_n p.p_hz (map base_act p.p_base) p.p_goal g w
+
+(** val elab : params -> gd gr list -> raw -> act list -> gd gr * act list **)
+
+let rec elab p ctx r acc =
+  match r with
+  | WEnd -> (REnd, acc)
+  | WAct (c, irr, p0, g) ->
+    let res = elab p ctx g acc in
+    if irr
+    then let cont = close ctx (skel p.p_worlds g) in
+         let hz_tbl = filter (fun w -> negb (gr0 p cont w)) p.p_worlds in
+         let b = nth c p.p_base never_b in
+         let ac = { a_pre = b.b_pre; a_add = b.b_add; a_del = b.b_del;
+           a_haz = hz_tbl }
+         in
+         ((RAct ((length (snd res)), p0, (fst res))),
+         (app (snd res) (ac :: [])))
+    else ((RAct (c, p0, (fst res))), (snd res))
+  | WChoice (p0, q, brs) ->
+    let res =
+      let rec go bs acc0 =
+        match bs with
+        | [] -> ([], acc0)
+        | b :: t ->
+          let r1 = elab p ctx (snd b) acc0 in
+          let g =
+            match snd (fst b) with
+            | Some f0 -> filter (fun w -> satf f0 w) p.p_worlds
+            | None ->
+              filter (fun w -> gr0 p (close ctx (skel p.p_worlds (snd b))) w)
+                p.p_worlds
+          in
+          let r2 = go t (snd r1) in
+          (((((fst (fst b)), g), (fst r1)) :: (fst r2)), (snd r2))
+      in go brs acc
+    in
+    ((RComm (p0, q, (fst res))), (snd res))
+  | WMu g ->
+    let res = elab p ((close ctx (RMu (skel p.p_worlds g))) :: ctx) g acc in
+    ((RMu (fst res)), (snd res))
+  | WVar i -> ((RVar i), acc)
+
+(** val reachable_worlds : params -> gd gr -> wd -> wd list **)
+
+let reachable_worlds p g0 w0 =
+  map snd
+    (iter' gW_dec (gsucc p.p_hz (map base_act p.p_base))
+      (length (list_prod (cands [] g0) p.p_worlds)) ((g0, w0) :: []))
+
+(** val kernel_run :
+    int -> bCap list -> f -> int list -> int -> raw -> int option **)
+
+let kernel_run n_atoms base goal init kmax raw0 =
+  let n = Stdlib.Int.succ n_atoms in
+  let all = all_bits n in
+  let w0 = set_all true init (repeat false n) in
+  let p0 = { p_n = n; p_hz = n_atoms; p_base = base; p_goal = goal;
+    p_worlds = all }
+  in
+  let ws = reachable_worlds p0 (skel all raw0) w0 in
+  let ws' = app ws (map (fun w -> wset w n_atoms true) ws) in
+  let p = { p_n = n; p_hz = n_atoms; p_base = base; p_goal = goal; p_worlds =
+    ws' }
+  in
+  let res = elab p [] raw0 (map base_act base) in
+  kernel_first n n_atoms (snd res) kmax (fst res) w0
