paper/WIP/proof/check_kernel.v
@@ -1,0 +1,4 @@
+Require Import Kernel.
+Print Assumptions kernel_correct.
+Print Assumptions kernel_first_spec.
+Print Assumptions goal_reachable_correct.
