paper/WIP/proof/extract.v
@@ -1,0 +1,4 @@
+Require Import Kernel.
+Require Import ExtrOcamlBasic ExtrOcamlNatInt.
+Extraction Blacklist List String.
+Extraction "kernel/kernel.ml" kernel_run.
